## Exercise 1

### Item (a)

For (X, Y, Z) = (a, b, Z), we have r(Y, X) = r(b, a) which is true, so not(r(Y, X)) is false.

For (X, Y, Z) = (a, c, Z), we have r(Y, X) = r(c, a) which can not be proven (and thus false), and s(Y, Y) = s(c, c), which is true.

For (X, Y, Z) = (b, a, Z), we have r(Y, X) = r(a, b) which is true.

For (X, Y, Z) = (a, d, Z), we have r(Y, X) = r(d, a) which can not be proven (and thus false), and s(Y, Y) = s(d, d) which can not be proven (and thus false as well); Thus, we choose the variable Z that appears first among the facts s(d, Z), which is s(d, e). Thus the first answer is (X, Y, Z) = (a, d, e).

### Item (b)

The interpreter backtracks 12 times before finding the first answer: 4 times for (X, Y) = (a, b), 4 times for (X, Y) = (a, c), and 4 times for (X, Y) = (b, a); it then finds an answer with (X, Y) = (a, d) without backtracking.
